Added Typechecking to compiler

01Source/Named.thy
@@ -14,18 +14,6 @@ primrec all_vars :: "nexpr \<Rightarrow> var set" where
 | "all_vars (NLam x e) = insert x (all_vars e)"
 | "all_vars (NApp e\<^sub>1 e\<^sub>2) = all_vars e\<^sub>1 \<union> all_vars e\<^sub>2"
 
-primrec binders :: "nexpr \<Rightarrow> var set" where
-  "binders (NVar x) = {}"
-| "binders (NConst k) = {}"
-| "binders (NLam x e) = insert x (binders e)"
-| "binders (NApp e\<^sub>1 e\<^sub>2) = binders e\<^sub>1 \<union> binders e\<^sub>2"
-
-primrec free_vars :: "nexpr \<Rightarrow> var set" where
-  "free_vars (NVar x) = {x}"
-| "free_vars (NConst k) = {}"
-| "free_vars (NLam x e) = free_vars e - {x}"
-| "free_vars (NApp e\<^sub>1 e\<^sub>2) = free_vars e\<^sub>1 \<union> free_vars e\<^sub>2"
-
 primrec valn :: "nexpr \<Rightarrow> bool" where
   "valn (NVar x) = False"
 | "valn (NConst k) = True" 
@@ -57,34 +45,7 @@ inductive evaln :: "nexpr \<Rightarrow> nexpr \<Rightarrow> bool" (infix "\<Down
 lemma [simp]: "finite (all_vars e)"
   by (induction e) simp_all
 
-lemma [simp]: "free_vars e \<subseteq> insert x xs \<Longrightarrow> free_vars (subst_var x x' e) \<subseteq> insert x' xs"
-proof (induction e arbitrary: xs)
-  case (NLam y e)
-  hence "free_vars e \<subseteq> insert x (insert y xs)" by auto
-  with NLam have "free_vars (subst_var x x' e) \<subseteq> insert x' (insert y xs)" by simp
-  with NLam show ?case by auto
-qed auto
-
-lemma free_vars_subst [simp]: "free_vars e \<subseteq> insert x xs \<Longrightarrow> free_vars e' \<subseteq> xs \<Longrightarrow> 
-  free_vars (substn x e' e) \<subseteq> xs"
-proof (induction x e' e arbitrary: xs rule: substn.induct)
-  case (3 x e' y e)
-  let ?z = "fresh (all_vars e' \<union> all_vars e \<union> {x, y})"
-  from 3 have "free_vars e \<subseteq> insert y (insert x xs)" by auto
-  hence "free_vars (subst_var y ?z e) \<subseteq> insert ?z (insert x xs)" by simp
-  hence "free_vars (subst_var y ?z e) \<subseteq> insert x (insert ?z xs)" by auto
-  with 3 show ?case by (auto simp add: Let_def)
-qed auto
-
-lemma free_vars_eval [simp]: "e \<Down> v \<Longrightarrow> free_vars e = {} \<Longrightarrow> free_vars v = {}"
-proof (induction e v rule: evaln.induct)
-  case (evn_app e\<^sub>1 x e\<^sub>1' e\<^sub>2 v\<^sub>2 v)
-  hence "free_vars e\<^sub>1' \<subseteq> insert x {} \<and> free_vars v\<^sub>2 \<subseteq> {}" by simp
-  hence "free_vars (substn x v\<^sub>2 e\<^sub>1') \<subseteq> {}" by (metis free_vars_subst)
-  with evn_app show ?case by simp
-qed simp_all
-
-(* We, obviously, do not have safety here yet. The relevant proofs are in 02/Named. *)
+(* We, obviously, do not have safety here yet. The relevant proofs are in 03Debruijn/NameRemoval. *)
 
 lemma [simp]: "e \<Down> v \<Longrightarrow> valn v"
   by (induction e v rule: evaln.induct) simp_all
