02Typed/Typed.thy
@@ -8,23 +8,17 @@ datatype texpr =
   | TLam var ty texpr
   | TApp texpr texpr
 
-primrec all_vars :: "texpr \<Rightarrow> var set" where
-  "all_vars (TVar x) = {x}"
-| "all_vars (TConst k) = {}"
-| "all_vars (TLam x t e) = insert x (all_vars e)"
-| "all_vars (TApp e\<^sub>1 e\<^sub>2) = all_vars e\<^sub>1 \<union> all_vars e\<^sub>2"
+primrec all_varst :: "texpr \<Rightarrow> var set" where
+  "all_varst (TVar x) = {x}"
+| "all_varst (TConst k) = {}"
+| "all_varst (TLam x t e) = insert x (all_varst e)"
+| "all_varst (TApp e\<^sub>1 e\<^sub>2) = all_varst e\<^sub>1 \<union> all_varst e\<^sub>2"
 
-primrec binders :: "texpr \<Rightarrow> var set" where
-  "binders (TVar x) = {}"
-| "binders (TConst k) = {}"
-| "binders (TLam x t e) = insert x (binders e)"
-| "binders (TApp e\<^sub>1 e\<^sub>2) = binders e\<^sub>1 \<union> binders e\<^sub>2"
-
-primrec free_vars :: "texpr \<Rightarrow> var set" where
-  "free_vars (TVar x) = {x}"
-| "free_vars (TConst k) = {}"
-| "free_vars (TLam x t e) = free_vars e - {x}"
-| "free_vars (TApp e\<^sub>1 e\<^sub>2) = free_vars e\<^sub>1 \<union> free_vars e\<^sub>2"
+primrec free_varst :: "texpr \<Rightarrow> var set" where
+  "free_varst (TVar x) = {x}"
+| "free_varst (TConst k) = {}"
+| "free_varst (TLam x t e) = free_varst e - {x}"
+| "free_varst (TApp e\<^sub>1 e\<^sub>2) = free_varst e\<^sub>1 \<union> free_varst e\<^sub>2"
 
 inductive typecheckn :: "(var \<rightharpoonup> ty) \<Rightarrow> texpr \<Rightarrow> ty \<Rightarrow> bool" (infix "\<turnstile>\<^sub>n _ :" 50) where
   tcn_var [simp]: "\<Gamma> x = Some t \<Longrightarrow> \<Gamma> \<turnstile>\<^sub>n TVar x : t"
@@ -37,130 +31,130 @@ inductive_cases [elim]: "\<Gamma> \<turnstile>\<^sub>n TConst k : t"
 inductive_cases [elim]: "\<Gamma> \<turnstile>\<^sub>n TLam x t' e : t"
 inductive_cases [elim]: "\<Gamma> \<turnstile>\<^sub>n TApp e\<^sub>1 e\<^sub>2 : t"
 
-primrec valn :: "texpr \<Rightarrow> bool" where
-  "valn (TVar x) = False"
-| "valn (TConst k) = True" 
-| "valn (TLam x t e) = True" 
-| "valn (TApp e\<^sub>1 e\<^sub>2) = False" 
+primrec valt :: "texpr \<Rightarrow> bool" where
+  "valt (TVar x) = False"
+| "valt (TConst k) = True" 
+| "valt (TLam x t e) = True" 
+| "valt (TApp e\<^sub>1 e\<^sub>2) = False" 
 
-primrec subst_var :: "var \<Rightarrow> var \<Rightarrow> texpr \<Rightarrow> texpr" where
-  "subst_var x x' (TVar y) = TVar (if x = y then x' else y)"
-| "subst_var x x' (TConst k) = TConst k"
-| "subst_var x x' (TLam y t e) = TLam y t (if x = y then e else subst_var x x' e)"
-| "subst_var x x' (TApp e\<^sub>1 e\<^sub>2) = TApp (subst_var x x' e\<^sub>1) (subst_var x x' e\<^sub>2)"
+primrec subst_vart :: "var \<Rightarrow> var \<Rightarrow> texpr \<Rightarrow> texpr" where
+  "subst_vart x x' (TVar y) = TVar (if x = y then x' else y)"
+| "subst_vart x x' (TConst k) = TConst k"
+| "subst_vart x x' (TLam y t e) = TLam y t (if x = y then e else subst_vart x x' e)"
+| "subst_vart x x' (TApp e\<^sub>1 e\<^sub>2) = TApp (subst_vart x x' e\<^sub>1) (subst_vart x x' e\<^sub>2)"
 
-lemma [simp]: "size (subst_var x x' e) = size e"
+lemma [simp]: "size (subst_vart x x' e) = size e"
   by (induction e) simp_all
 
-fun substn :: "var \<Rightarrow> texpr \<Rightarrow> texpr \<Rightarrow> texpr" where
-  "substn x e' (TVar y) = (if x = y then e' else TVar y)"
-| "substn x e' (TConst k) = TConst k"
-| "substn x e' (TLam y t e) = (
-    let z = fresh (all_vars e' \<union> all_vars e \<union> {x, y})
-    in TLam z t (substn x e' (subst_var y z e)))"
-| "substn x e' (TApp e\<^sub>1 e\<^sub>2) = TApp (substn x e' e\<^sub>1) (substn x e' e\<^sub>2)"
+fun substt :: "var \<Rightarrow> texpr \<Rightarrow> texpr \<Rightarrow> texpr" where
+  "substt x e' (TVar y) = (if x = y then e' else TVar y)"
+| "substt x e' (TConst k) = TConst k"
+| "substt x e' (TLam y t e) = (
+    let z = fresh (all_varst e' \<union> all_varst e \<union> {x, y})
+    in TLam z t (substt x e' (subst_vart y z e)))"
+| "substt x e' (TApp e\<^sub>1 e\<^sub>2) = TApp (substt x e' e\<^sub>1) (substt x e' e\<^sub>2)"
 
-inductive evaln :: "texpr \<Rightarrow> texpr \<Rightarrow> bool" (infix "\<Down>" 50) where
-  evn_const [simp]: "TConst k \<Down> TConst k"
-| evn_lam [simp]: "TLam x t e \<Down> TLam x t e"
-| evn_app [simp]: "e\<^sub>1 \<Down> TLam x t e\<^sub>1' \<Longrightarrow> e\<^sub>2 \<Down> v\<^sub>2 \<Longrightarrow> substn x v\<^sub>2 e\<^sub>1' \<Down> v \<Longrightarrow> TApp e\<^sub>1 e\<^sub>2 \<Down> v"
+inductive evalt :: "texpr \<Rightarrow> texpr \<Rightarrow> bool" (infix "\<Down>\<^sub>t" 50) where
+  evt_const [simp]: "TConst k \<Down>\<^sub>t TConst k"
+| evt_lam [simp]: "TLam x t e \<Down>\<^sub>t TLam x t e"
+| evt_app [simp]: "e\<^sub>1 \<Down>\<^sub>t TLam x t e\<^sub>1' \<Longrightarrow> e\<^sub>2 \<Down>\<^sub>t v\<^sub>2 \<Longrightarrow> substt x v\<^sub>2 e\<^sub>1' \<Down>\<^sub>t v \<Longrightarrow> TApp e\<^sub>1 e\<^sub>2 \<Down>\<^sub>t v"
 
-lemma [simp]: "finite (all_vars e)"
+lemma [simp]: "finite (all_varst e)"
   by (induction e) simp_all
 
-lemma [simp]: "free_vars e \<subseteq> insert x xs \<Longrightarrow> free_vars (subst_var x x' e) \<subseteq> insert x' xs"
+lemma [simp]: "free_varst e \<subseteq> insert x xs \<Longrightarrow> free_varst (subst_vart x x' e) \<subseteq> insert x' xs"
 proof (induction e arbitrary: xs)
   case (TLam y t e)
-  hence "free_vars e \<subseteq> insert x (insert y xs)" by auto
-  with TLam have "free_vars (subst_var x x' e) \<subseteq> insert x' (insert y xs)" by simp
+  hence "free_varst e \<subseteq> insert x (insert y xs)" by auto
+  with TLam have "free_varst (subst_vart x x' e) \<subseteq> insert x' (insert y xs)" by simp
   with TLam show ?case by auto
 qed auto
 
-lemma free_vars_subst [simp]: "free_vars e \<subseteq> insert x xs \<Longrightarrow> free_vars e' \<subseteq> xs \<Longrightarrow> 
-  free_vars (substn x e' e) \<subseteq> xs"
-proof (induction x e' e arbitrary: xs rule: substn.induct)
+lemma free_vars_substt [simp]: "free_varst e \<subseteq> insert x xs \<Longrightarrow> free_varst e' \<subseteq> xs \<Longrightarrow> 
+  free_varst (substt x e' e) \<subseteq> xs"
+proof (induction x e' e arbitrary: xs rule: substt.induct)
   case (3 x e' y t e)
-  let ?z = "fresh (all_vars e' \<union> all_vars e \<union> {x, y})"
-  from 3 have "free_vars e \<subseteq> insert y (insert x xs)" by auto
-  hence "free_vars (subst_var y ?z e) \<subseteq> insert ?z (insert x xs)" by simp
-  hence "free_vars (subst_var y ?z e) \<subseteq> insert x (insert ?z xs)" by auto
+  let ?z = "fresh (all_varst e' \<union> all_varst e \<union> {x, y})"
+  from 3 have "free_varst e \<subseteq> insert y (insert x xs)" by auto
+  hence "free_varst (subst_vart y ?z e) \<subseteq> insert ?z (insert x xs)" by simp
+  hence "free_varst (subst_vart y ?z e) \<subseteq> insert x (insert ?z xs)" by auto
   with 3 show ?case by (auto simp add: Let_def)
 qed auto
 
-lemma free_vars_eval [simp]: "e \<Down> v \<Longrightarrow> free_vars e = {} \<Longrightarrow> free_vars v = {}"
-proof (induction e v rule: evaln.induct)
-  case (evn_app e\<^sub>1 x t e\<^sub>1' e\<^sub>2 v\<^sub>2 v)
-  hence "free_vars e\<^sub>1' \<subseteq> insert x {} \<and> free_vars v\<^sub>2 \<subseteq> {}" by simp
-  hence "free_vars (substn x v\<^sub>2 e\<^sub>1') \<subseteq> {}" by (metis free_vars_subst)
-  with evn_app show ?case by simp
+lemma free_vars_evalt [simp]: "e \<Down>\<^sub>t v \<Longrightarrow> free_varst e = {} \<Longrightarrow> free_varst v = {}"
+proof (induction e v rule: evalt.induct)
+  case (evt_app e\<^sub>1 x t e\<^sub>1' e\<^sub>2 v\<^sub>2 v)
+  hence "free_varst e\<^sub>1' \<subseteq> insert x {} \<and> free_varst v\<^sub>2 \<subseteq> {}" by simp
+  hence "free_varst (substt x v\<^sub>2 e\<^sub>1') \<subseteq> {}" by (metis free_vars_substt)
+  with evt_app show ?case by simp
 qed simp_all
 
-lemma free_vars_subs [simp]: "\<Gamma> \<turnstile>\<^sub>n e : t \<Longrightarrow> free_vars e \<subseteq> dom \<Gamma>" 
+lemma free_vars_subs [simp]: "\<Gamma> \<turnstile>\<^sub>n e : t \<Longrightarrow> free_varst e \<subseteq> dom \<Gamma>" 
   by (induction \<Gamma> e t rule: typecheckn.induct) auto
 
-lemma [simp]: "Map.empty \<turnstile>\<^sub>n e : t \<Longrightarrow> free_vars e = {}"
+lemma [simp]: "Map.empty \<turnstile>\<^sub>n e : t \<Longrightarrow> free_varst e = {}"
   using free_vars_subs by fastforce
 
-lemma canonical_basen [dest]: "\<Gamma> \<turnstile>\<^sub>n e : Base \<Longrightarrow> valn e \<Longrightarrow> \<exists>k. e = TConst k"
+lemma canonical_basen [dest]: "\<Gamma> \<turnstile>\<^sub>n e : Base \<Longrightarrow> valt e \<Longrightarrow> \<exists>k. e = TConst k"
   by (induction \<Gamma> e Base rule: typecheckn.induct) simp_all
 
-lemma canonical_arrown [dest]: "\<Gamma> \<turnstile>\<^sub>n e : Arrow t\<^sub>1 t\<^sub>2 \<Longrightarrow> valn e \<Longrightarrow> 
+lemma canonical_arrown [dest]: "\<Gamma> \<turnstile>\<^sub>n e : Arrow t\<^sub>1 t\<^sub>2 \<Longrightarrow> valt e \<Longrightarrow> 
     \<exists>x e'. e = TLam x t\<^sub>1 e' \<and> \<Gamma>(x \<mapsto> t\<^sub>1) \<turnstile>\<^sub>n e' : t\<^sub>2"
   by (induction \<Gamma> e "Arrow t\<^sub>1 t\<^sub>2" rule: typecheckn.induct) simp_all
 
 (* Progress not directly provable here, due to lack of proof of termination.
    We prove it in 02Debruijn/NameRemoval *)
 
-lemma [simp]: "\<Gamma> \<turnstile>\<^sub>n e : t \<Longrightarrow> x \<notin> all_vars e \<Longrightarrow> \<Gamma>(x \<mapsto> t') \<turnstile>\<^sub>n e : t"
+lemma [simp]: "\<Gamma> \<turnstile>\<^sub>n e : t \<Longrightarrow> x \<notin> all_varst e \<Longrightarrow> \<Gamma>(x \<mapsto> t') \<turnstile>\<^sub>n e : t"
   by (induction \<Gamma> e t rule: typecheckn.induct) (simp_all add: fun_upd_twist)
 
-lemma [simp]: "\<Gamma>(x \<mapsto> t') \<turnstile>\<^sub>n e : t \<Longrightarrow> x' \<notin> all_vars e \<Longrightarrow> \<Gamma>(x' \<mapsto> t') \<turnstile>\<^sub>n subst_var x x' e : t"
+lemma [simp]: "\<Gamma>(x \<mapsto> t') \<turnstile>\<^sub>n e : t \<Longrightarrow> x' \<notin> all_varst e \<Longrightarrow> \<Gamma>(x' \<mapsto> t') \<turnstile>\<^sub>n subst_vart x x' e : t"
 proof (induction "\<Gamma>(x \<mapsto> t')" e t arbitrary: \<Gamma> rule: typecheckn.induct)
   case (tcn_lam y t\<^sub>1 e t\<^sub>2)
   thus ?case
   proof (cases "x = y")
     case False
-    moreover with tcn_lam have "\<Gamma>(y \<mapsto> t\<^sub>1, x' \<mapsto> t') \<turnstile>\<^sub>n subst_var x x' e : t\<^sub>2" 
+    moreover with tcn_lam have "\<Gamma>(y \<mapsto> t\<^sub>1, x' \<mapsto> t') \<turnstile>\<^sub>n subst_vart x x' e : t\<^sub>2" 
       by (simp add: fun_upd_twist)
     moreover from tcn_lam have "x' \<noteq> y" by simp
     ultimately show ?thesis by (simp add: fun_upd_twist)
   qed (simp_all add: fun_upd_twist)
 qed fastforce+
 
-lemma [simp]: "\<Gamma>(x \<mapsto> t') \<turnstile>\<^sub>n e : t \<Longrightarrow> \<Gamma> \<turnstile>\<^sub>n e' : t' \<Longrightarrow> \<Gamma> \<turnstile>\<^sub>n substn x e' e : t"
-proof (induction x e' e arbitrary: \<Gamma> t rule: substn.induct)
+lemma [simp]: "\<Gamma>(x \<mapsto> t') \<turnstile>\<^sub>n e : t \<Longrightarrow> \<Gamma> \<turnstile>\<^sub>n e' : t' \<Longrightarrow> \<Gamma> \<turnstile>\<^sub>n substt x e' e : t"
+proof (induction x e' e arbitrary: \<Gamma> t rule: substt.induct)
   case (3 x e' y t\<^sub>1 e)
   then obtain t\<^sub>2 where T: "t = Arrow t\<^sub>1 t\<^sub>2 \<and> \<Gamma>(x \<mapsto> t', y \<mapsto> t\<^sub>1) \<turnstile>\<^sub>n e : t\<^sub>2" by blast
-  let ?z = "fresh (all_vars e' \<union> all_vars e \<union> {x, y})"
-  have "finite (all_vars e' \<union> all_vars e \<union> {x, y})" by simp
-  hence Z: "?z \<notin> all_vars e' \<union> all_vars e \<union> {x, y}" by (metis fresh_is_fresh)
-  with T have "\<Gamma>(x \<mapsto> t', ?z \<mapsto> t\<^sub>1) \<turnstile>\<^sub>n subst_var y ?z e : t\<^sub>2" by simp
-  with Z have X: "\<Gamma>(?z \<mapsto> t\<^sub>1, x \<mapsto> t') \<turnstile>\<^sub>n subst_var y ?z e : t\<^sub>2" by (simp add: fun_upd_twist)
+  let ?z = "fresh (all_varst e' \<union> all_varst e \<union> {x, y})"
+  have "finite (all_varst e' \<union> all_varst e \<union> {x, y})" by simp
+  hence Z: "?z \<notin> all_varst e' \<union> all_varst e \<union> {x, y}" by (metis fresh_is_fresh)
+  with T have "\<Gamma>(x \<mapsto> t', ?z \<mapsto> t\<^sub>1) \<turnstile>\<^sub>n subst_vart y ?z e : t\<^sub>2" by simp
+  with Z have X: "\<Gamma>(?z \<mapsto> t\<^sub>1, x \<mapsto> t') \<turnstile>\<^sub>n subst_vart y ?z e : t\<^sub>2" by (simp add: fun_upd_twist)
   from 3 Z have "\<Gamma>(?z \<mapsto> t\<^sub>1) \<turnstile>\<^sub>n e' : t'" by simp
-  with 3 X have "\<Gamma>(?z \<mapsto> t\<^sub>1) \<turnstile>\<^sub>n substn x e' (subst_var y ?z e) : t\<^sub>2" by fastforce
+  with 3 X have "\<Gamma>(?z \<mapsto> t\<^sub>1) \<turnstile>\<^sub>n substt x e' (subst_vart y ?z e) : t\<^sub>2" by fastforce
   with T show ?case by (simp add: Let_def)
 qed fastforce+
 
-theorem preservationn: "e \<Down> v \<Longrightarrow> \<Gamma> \<turnstile>\<^sub>n e : t \<Longrightarrow> \<Gamma> \<turnstile>\<^sub>n v : t"
-  by (induction e v arbitrary: t rule: evaln.induct) fastforce+
+theorem preservationn: "e \<Down>\<^sub>t v \<Longrightarrow> \<Gamma> \<turnstile>\<^sub>n e : t \<Longrightarrow> \<Gamma> \<turnstile>\<^sub>n v : t"
+  by (induction e v arbitrary: t rule: evalt.induct) fastforce+
 
-lemma [simp]: "e \<Down> v \<Longrightarrow> valn v"
-  by (induction e v rule: evaln.induct) simp_all
+lemma [simp]: "e \<Down>\<^sub>t v \<Longrightarrow> valt v"
+  by (induction e v rule: evalt.induct) simp_all
 
-lemma val_no_evaln: "e \<Down> v \<Longrightarrow> valn e \<Longrightarrow> v = e"
-  by (induction e v rule: evaln.induct) simp_all
+lemma val_no_evaln: "e \<Down>\<^sub>t v \<Longrightarrow> valt e \<Longrightarrow> v = e"
+  by (induction e v rule: evalt.induct) simp_all
 
-theorem determinismn: "e \<Down> v \<Longrightarrow> e \<Down> v' \<Longrightarrow> v = v'"
-proof (induction e v arbitrary: v' rule: evaln.induct)
-  case (evn_const k)
-  thus ?case by (induction "TConst k" v' rule: evaln.induct) simp_all
+theorem determinismn: "e \<Down>\<^sub>t v \<Longrightarrow> e \<Down>\<^sub>t v' \<Longrightarrow> v = v'"
+proof (induction e v arbitrary: v' rule: evalt.induct)
+  case (evt_const k)
+  thus ?case by (induction "TConst k" v' rule: evalt.induct) simp_all
 next
-  case (evn_lam x t e)
-  thus ?case by (induction "TLam x t e" v' rule: evaln.induct) simp_all
+  case (evt_lam x t e)
+  thus ?case by (induction "TLam x t e" v' rule: evalt.induct) simp_all
 next
-  case (evn_app e\<^sub>1 x t e\<^sub>1' e\<^sub>2 v\<^sub>2 v)
-  from evn_app(7, 1, 2, 3, 4, 5, 6) show ?case 
-    by (induction "TApp e\<^sub>1 e\<^sub>2" v' rule: evaln.induct) blast+
+  case (evt_app e\<^sub>1 x t e\<^sub>1' e\<^sub>2 v\<^sub>2 v)
+  from evt_app(7, 1, 2, 3, 4, 5, 6) show ?case 
+    by (induction "TApp e\<^sub>1 e\<^sub>2" v' rule: evalt.induct) blast+
 qed
 
 end
