Compiler.thy
@@ -2,43 +2,53 @@ theory Compiler
   imports Printing "04Stack/StackConversion" "12UnstructuredMemory/Unstructuring" 
 begin
 
-abbreviation compile :: "texpr \<Rightarrow> byte_code list" where 
-  "compile \<equiv> flatten_code \<circ> tco \<circ> encode \<circ> convert"
+abbreviation compile :: "nexpr \<rightharpoonup> byte_code list" where 
+  "compile \<equiv> map_option (flatten_code \<circ> tco \<circ> encode \<circ> convert \<circ> fst) \<circ> typecheck"
 
 lemma [simp]: "live_frame (env, tco_cd (encode e), tco_r (encode e))"
   by (induction e) simp_all
 
-theorem tc_terminationn: "\<exists>t. Map.empty \<turnstile>\<^sub>n e : t \<Longrightarrow> compile e = cd \<Longrightarrow> 
+theorem tc_failure: "compile e = None \<Longrightarrow> \<nexists>e\<^sub>t t. (Map.empty \<turnstile>\<^sub>n e\<^sub>t : t) \<and> e = erase e\<^sub>t"
+proof -
+  assume "compile e = None"
+  hence "typecheck e = None" by simp
+  thus ?thesis by (metis typecheck_fails)
+qed
+
+theorem tc_terminationn: "compile e = Some cd \<Longrightarrow> 
   \<exists>v. valn v \<and> e \<Down> v \<and> 
     (\<exists>h hp e ep v\<^sub>u s. iter (\<leadsto>\<^sub>u) (US nmem 0 0 0 nmem 0 nmem 0 (nmem(0 := 0)) 1 (length cd) cd) 
-      (US h hp 0 0 e ep v\<^sub>u 1 s 0 0 cd) \<and> print_uclosure h (v\<^sub>u 0) = print_texpr v)"
+      (US h hp 0 0 e ep v\<^sub>u 1 s 0 0 cd) \<and> print_uclosure h (v\<^sub>u 0) = print_nexpr v)"
 proof -
-  assume "\<exists>t. Map.empty \<turnstile>\<^sub>n e : t"
-  then obtain t where TN: "Map.empty \<turnstile>\<^sub>n e : t" by fastforce
-  then obtain v\<^sub>n where EN: "e \<Down> v\<^sub>n" by fastforce
-  hence VN: "valn v\<^sub>n" by simp
-  from TN have TD: "[] \<turnstile>\<^sub>d convert e : t" by simp
-  from EN TN have ED: "convert e \<Down>\<^sub>d convert v\<^sub>n" by simp
-  hence VD: "vald (convert v\<^sub>n)" by simp
-  from ED have "iter (\<leadsto>\<^sub>d) (convert e) (convert v\<^sub>n)" by (metis BigStep.correctb)
-  with ED EN TD have ES: "iter (\<leadsto>\<^sub>s) (SS False [FReturn] (convert e)) (SS True [] (convert v\<^sub>n))" 
+  assume C: "compile e = Some cd"
+  then obtain e\<^sub>t t where T: "typecheck e = Some (e\<^sub>t, t)" by fastforce
+  hence TN: "(Map.empty \<turnstile>\<^sub>n e\<^sub>t : t) \<and> e = erase e\<^sub>t" by simp
+  then obtain v\<^sub>t where ET: "e\<^sub>t \<Down>\<^sub>t v\<^sub>t" by fastforce
+  hence VT: "valt v\<^sub>t" by simp
+  hence VN: "valn (erase v\<^sub>t)" by simp
+  from ET have EN: "erase e\<^sub>t \<Down> erase v\<^sub>t" by simp
+  from TN have TD: "[] \<turnstile>\<^sub>d convert e\<^sub>t : t" by simp
+  from ET TN have ED: "convert e\<^sub>t \<Down>\<^sub>d convert v\<^sub>t" by fastforce
+  hence VD: "vald (convert v\<^sub>t)" by simp
+  from ED have "iter (\<leadsto>\<^sub>d) (convert e\<^sub>t) (convert v\<^sub>t)" by (metis BigStep.correctb)
+  with ED EN TD have ES: "iter (\<leadsto>\<^sub>s) (SS False [FReturn] (convert e\<^sub>t)) (SS True [] (convert v\<^sub>t))" 
     by simp
-  from TD have TC: "CSE [CReturn []] [] (convert e) :\<^sub>c t" 
+  from TD have TC: "CSE [CReturn []] [] (convert e\<^sub>t) :\<^sub>c t" 
     by (metis tcc_state_ev tcc_nil tcc_snil tcc_scons_ret latest_environment.simps(4))
-  with ES VD EN obtain c where EC: "iter (\<leadsto>\<^sub>c) (CSE [CReturn []] [] (convert e)) (CSC [] c) \<and> 
-    declosure c = convert v\<^sub>n" by fastforce
-  with VN have VC: "print_closure c = print_texpr v\<^sub>n" by simp
-  from TC EC have "iter (\<leadsto>\<^sub>t) (encode_state (CSE [CReturn []] [] (convert e))) 
+  with ES VD EN obtain c where EC: "iter (\<leadsto>\<^sub>c) (CSE [CReturn []] [] (convert e\<^sub>t)) (CSC [] c) \<and> 
+    declosure c = convert v\<^sub>t" by fastforce
+  with VT have VC: "print_closure c = print_nexpr (erase v\<^sub>t)" by simp
+  from TC EC have "iter (\<leadsto>\<^sub>t) (encode_state (CSE [CReturn []] [] (convert e\<^sub>t))) 
     (encode_state (CSC [] c))" by (metis iter_completet)
-  hence "iter (\<leadsto>\<^sub>t) (TS [] [([], encode (convert e))]) (TS [encode_closure c] [])" 
+  hence "iter (\<leadsto>\<^sub>t) (TS [] [([], encode (convert e\<^sub>t))]) (TS [encode_closure c] [])" 
     by (simp add: encode_def)
-  hence "iter (\<leadsto>\<^sub>t\<^sub>c\<^sub>o) (tco_state (TS [] [([], encode (convert e))])) 
+  hence "iter (\<leadsto>\<^sub>t\<^sub>c\<^sub>o) (tco_state (TS [] [([], encode (convert e\<^sub>t))])) 
     (tco_state (TS [encode_closure c] []))" by (metis iter_tco_eval)
-  hence ET: "iter (\<leadsto>\<^sub>t\<^sub>c\<^sub>o) (TCOS [] [([], tco_cd (encode (convert e)), tco_r (encode (convert e)))]) 
+  hence ET: "iter (\<leadsto>\<^sub>t\<^sub>c\<^sub>o) (TCOS [] [([], tco_cd (encode (convert e\<^sub>t)), tco_r (encode (convert e\<^sub>t)))]) 
     (TCOS [tco_val (encode_closure c)] [])" by simp
-  assume C: "compile e = cd"
+  from C T have "(flatten_code \<circ> tco \<circ> encode \<circ> convert) e\<^sub>t = cd" by simp
   hence UB: "unflatten_state (BS [] [([], length cd)] cd) = 
-    TCOS [] [([], tco_cd (encode (convert e)), tco_r (encode (convert e)))]" 
+    TCOS [] [([], tco_cd (encode (convert e\<^sub>t)), tco_r (encode (convert e\<^sub>t)))]" 
       by (auto simp add: tco_def simp del: flatten_code.simps)
   from C have "orderly_state (BS [] [([], length cd)] cd)" by auto
   with ET UB obtain v\<^sub>b where EB: 
@@ -46,12 +56,12 @@ proof -
       tco_val (encode_closure c) = unflatten_closure cd v\<^sub>b" 
     by (metis evalb_end byte_code_state.sel(3))
   hence "print_bclosure v\<^sub>b = print_tco_closure (tco_val (encode_closure c))" by simp
-  with VC have VB: "print_bclosure v\<^sub>b = print_texpr v\<^sub>n" by simp
+  with VC have VB: "print_bclosure v\<^sub>b = print_nexpr (erase v\<^sub>t)" by simp
   from EB obtain \<Sigma>\<^sub>h' where EH: "iter (\<leadsto>\<^sub>h) (HS hempty [] [([], length cd)] cd) \<Sigma>\<^sub>h' \<and> 
     BS [v\<^sub>b] [] cd = unheap \<Sigma>\<^sub>h'" by fastforce
   then obtain h\<^sub>h v\<^sub>h where SH: "\<Sigma>\<^sub>h' = HS h\<^sub>h [v\<^sub>h] [] cd \<and> v\<^sub>b = unheap_closure h\<^sub>h v\<^sub>h" 
     using unheap_empty by blast
-  with VB have VH: "print_hclosure (hlookup h\<^sub>h v\<^sub>h) = print_texpr v\<^sub>n" by simp
+  with VB have VH: "print_hclosure (hlookup h\<^sub>h v\<^sub>h) = print_nexpr (erase v\<^sub>t)" by simp
   have HS: "heap_structured (HS hempty [] [([], length cd)] cd)" by simp
   have CES: "unchain_state (CES hempty hempty [] [(0, length cd)] cd) = 
     HS hempty [] [([], length cd)] cd" by simp
@@ -59,12 +69,12 @@ proof -
     HS h\<^sub>h [v\<^sub>h] [] cd = unchain_state \<Sigma>\<^sub>c\<^sub>e'" by fastforce
   then obtain h\<^sub>c\<^sub>e env\<^sub>h where VCE: "\<Sigma>\<^sub>c\<^sub>e' = CES h\<^sub>c\<^sub>e env\<^sub>h [v\<^sub>h] [] cd \<and> h\<^sub>h = unchain_heap h\<^sub>c\<^sub>e env\<^sub>h" 
     by (metis unchain_state_reverse map_is_Nil_conv)
-  with VH have PCE: "print_ceclosure (hlookup h\<^sub>c\<^sub>e v\<^sub>h) = print_texpr v\<^sub>n" by (metis print_ce)
+  with VH have PCE: "print_ceclosure (hlookup h\<^sub>c\<^sub>e v\<^sub>h) = print_nexpr (erase v\<^sub>t)" by (metis print_ce)
   from ECE VCE have "iter (\<leadsto>\<^sub>f) (flatten (CES hempty hempty [] [(0, length cd)] cd))
     (flatten (CES h\<^sub>c\<^sub>e env\<^sub>h [v\<^sub>h] [] cd))" by (metis completef_iter)
   hence EF: "iter (\<leadsto>\<^sub>f) (FS (H nmem 0) (H nmem 0) [] [length cd, 0] cd)
      (FS (flatten_values h\<^sub>c\<^sub>e) (flatten_environment env\<^sub>h) [v\<^sub>h] [] cd)" by (simp add: hempty_def)
-  from PCE have PF: "print_ceclosure (get_closure (flatten_values h\<^sub>c\<^sub>e) v\<^sub>h) = print_texpr v\<^sub>n" 
+  from PCE have PF: "print_ceclosure (get_closure (flatten_values h\<^sub>c\<^sub>e) v\<^sub>h) = print_nexpr (erase v\<^sub>t)" 
     by (simp del: get_closure.simps)
   from C have "cd \<noteq> []" by auto
   with EF have "\<exists>\<Sigma>\<^sub>u'. iter (\<leadsto>\<^sub>u) (US nmem 0 0 0 nmem 0 nmem 0 (nmem(0 := 0)) 1 (length cd) cd) \<Sigma>\<^sub>u' \<and> 
@@ -85,12 +95,11 @@ proof -
 
 
 
-  from PF VU VSU have PU: "print_uclosure h\<^sub>u (vs\<^sub>u 0) = print_texpr v\<^sub>n" by (metis print_u)
+  from PF VU VSU have PU: "print_uclosure h\<^sub>u (vs\<^sub>u 0) = print_nexpr (erase v\<^sub>t)" by (metis print_u)
 
 
 
-
-  with EN EU VN PU show ?thesis by blast
+  with VN TN EN EU PU show ?thesis by blast
 qed
 
 end
