02Typed/Typechecking.thy
@@ -1,0 +1,41 @@
+theory Typechecking
+  imports Typed "../01Source/Named" "../00Utils/Unification/Unification"
+begin
+
+primrec erase :: "texpr \<Rightarrow> nexpr" where
+  "erase (TVar x) = NVar x"
+| "erase (TConst k) = NConst k"
+| "erase (TLam x t e) = NLam x (erase e)"
+| "erase (TApp e\<^sub>1 e\<^sub>2) = NApp (erase e\<^sub>1) (erase e\<^sub>2)"
+
+primrec typecheck :: "nexpr \<rightharpoonup> texpr \<times> ty" where
+  "typecheck (NVar x) = undefined"
+
+lemma [simp]: "typecheck e = Some (e\<^sub>t, t) \<Longrightarrow> Map.empty \<turnstile>\<^sub>n e\<^sub>t : t"
+  by simp
+
+lemma [simp]: "typecheck e = Some (e\<^sub>t, t) \<Longrightarrow> e = erase e\<^sub>t"
+  by simp
+
+lemma typecheck_fails [simp]: "typecheck e = None \<Longrightarrow> \<nexists>e\<^sub>t t. (Map.empty \<turnstile>\<^sub>n e\<^sub>t : t) \<and> e = erase e\<^sub>t"
+  by simp
+
+lemma [simp]: "valn (erase e) = valt e"
+  by (induction e) simp_all
+
+lemma [simp]: "all_vars (erase e) = all_varst e"
+  by (induction e) simp_all
+
+lemma [simp]: "erase (subst_vart x y e) = subst_var x y (erase e)"
+  by (induction e) simp_all
+
+lemma [simp]: "erase (substt x e' e) = substn x (erase e') (erase e)"
+  by (induction x e' e rule: substt.induct) (simp_all add: Let_def)
+
+theorem completeness [simp]: "e \<Down>\<^sub>t v \<Longrightarrow> erase e \<Down> erase v"
+  by (induction e v rule: evalt.induct) simp_all
+
+theorem correctness: "e \<Down> v \<Longrightarrow> typecheck e = Some (e\<^sub>t, t) \<Longrightarrow> typecheck v = Some (v\<^sub>t, t) \<Longrightarrow> e\<^sub>t \<Down>\<^sub>t v\<^sub>t"
+  by (induction e v rule: evaln.induct) simp_all
+
+end
